backend/MachineModelLow.v
@@ -53,7 +53,6 @@ Definition me_query (me : machine_env) (q: state_query) : val :=
   | Qcall0 Btimestamp => Vint (me_timestamp me)
   | Qcall0 Bnumber => Vint (me_number me)
   | Qcall0 Bchainid => Vint (me_chainid me)
-  | Qcall0 Bselfbalance => Vint (me_selfbalance me)
   | Qcall1 Bbalance (Vint addr) => Vint (me_balance me addr)
   | Qcall1 Bbalance _ => Vunit (* ill-typed query. *)
   | Qcall1 Bblockhash (Vint n) => Vint (me_blockhash me n)
