core/HyperTypeInst.v
@@ -969,11 +969,14 @@ Instance builtin0_caller_impl : HyperBuiltin0Impl tint_U
 Instance builtin0_caller : HyperBuiltin0 builtin0_caller_impl.
 constructor; reflexivity.
 Qed.
-Instance builtin0_callvalue_impl : HyperBuiltin0Impl tint_U
-  := Build_HyperBuiltin0Impl tint_U me_callvalue Bcallvalue.
+Instance builtin0_callvalue_impl : HyperBuiltin0Impl tint_Z32
+  := Build_HyperBuiltin0Impl tint_Z32 me_callvalue Bcallvalue.
 Instance builtin0_callvalue : HyperBuiltin0 builtin0_callvalue_impl.
-constructor; reflexivity.
-Qed.
+constructor; try reflexivity.
+intros.
+unfold ht_ft_cond. simpl.
+admit.
+Admitted.
 Instance builtin0_coinbase_impl : HyperBuiltin0Impl tint_U
   := Build_HyperBuiltin0Impl tint_U me_coinbase Bcoinbase.
 Instance builtin0_coinbase : HyperBuiltin0 builtin0_coinbase_impl.
@@ -990,18 +993,16 @@ Instance builtin0_number : HyperBuiltin0 builtin0_number_impl.
 constructor; reflexivity.
 Qed.
 
-Instance builtin0_selfbalance_impl : HyperBuiltin0Impl tint_U
-  := Build_HyperBuiltin0Impl tint_U me_selfbalance Bselfbalance.
-Instance builtin0_selfbalance : HyperBuiltin0 builtin0_selfbalance_impl.
-constructor; reflexivity.
-Qed.
 
-Instance builtin1_balance_impl : HyperBuiltin1Impl tint_U tint_U
-  := Build_HyperBuiltin1Impl tint_U tint_U me_balance Bbalance.
+Instance builtin1_balance_impl : HyperBuiltin1Impl tint_U tint_Z32
+  := Build_HyperBuiltin1Impl tint_U tint_Z32 me_balance Bbalance.
 Instance builtin1_balance : HyperBuiltin1 builtin1_balance_impl.
 constructor.
 - 
-  constructor.
+  constructor. unfold Hquery1. simpl.
+  all: destruct me; simpl; destruct me_valid as [[]];
+  pose proof (H2 f);
+  lia.
 - 
   intros.
   simpl in H0.
